linux/pkvm/proofs/early_alloc/generated_code.v
@@ -6,95 +6,100 @@ Set Default Proof Using "Type".
 (* Generated from [linux/pkvm/early_alloc.c]. *)
 Section code.
   Definition file_0 : string := "linux/pkvm/early_alloc.c".
-  Definition loc_2 : location_info := LocationInfo file_0 39 2 39 52.
-  Definition loc_3 : location_info := LocationInfo file_0 39 9 39 51.
-  Definition loc_4 : location_info := LocationInfo file_0 39 9 39 45.
-  Definition loc_5 : location_info := LocationInfo file_0 39 10 39 19.
-  Definition loc_6 : location_info := LocationInfo file_0 39 10 39 19.
-  Definition loc_7 : location_info := LocationInfo file_0 39 11 39 14.
-  Definition loc_8 : location_info := LocationInfo file_0 39 22 39 44.
-  Definition loc_9 : location_info := LocationInfo file_0 39 34 39 44.
-  Definition loc_10 : location_info := LocationInfo file_0 39 34 39 44.
-  Definition loc_11 : location_info := LocationInfo file_0 39 35 39 38.
-  Definition loc_12 : location_info := LocationInfo file_0 39 49 39 51.
-  Definition loc_15 : location_info := LocationInfo file_0 55 2 55 31.
-  Definition loc_16 : location_info := LocationInfo file_0 58 2 59 26.
-  Definition loc_17 : location_info := LocationInfo file_0 61 2 61 30.
-  Definition loc_18 : location_info := LocationInfo file_0 62 2 65 3.
-  Definition loc_19 : location_info := LocationInfo file_0 73 2 73 67.
-  Definition loc_20 : location_info := LocationInfo file_0 73 9 73 66.
-  Definition loc_21 : location_info := LocationInfo file_0 73 35 73 47.
-  Definition loc_22 : location_info := LocationInfo file_0 73 35 73 47.
-  Definition loc_23 : location_info := LocationInfo file_0 73 37 73 40.
-  Definition loc_24 : location_info := LocationInfo file_0 73 51 73 65.
-  Definition loc_25 : location_info := LocationInfo file_0 73 61 73 64.
-  Definition loc_26 : location_info := LocationInfo file_0 73 61 73 64.
-  Definition loc_27 : location_info := LocationInfo file_0 62 29 65 3.
-  Definition loc_28 : location_info := LocationInfo file_0 63 4 63 20.
-  Definition loc_29 : location_info := LocationInfo file_0 64 4 64 26.
-  Definition loc_30 : location_info := LocationInfo file_0 64 11 64 25.
-  Definition loc_31 : location_info := LocationInfo file_0 63 4 63 13.
-  Definition loc_32 : location_info := LocationInfo file_0 63 5 63 8.
-  Definition loc_33 : location_info := LocationInfo file_0 63 16 63 19.
-  Definition loc_34 : location_info := LocationInfo file_0 63 16 63 19.
-  Definition loc_36 : location_info := LocationInfo file_0 62 6 62 27.
-  Definition loc_37 : location_info := LocationInfo file_0 62 6 62 15.
-  Definition loc_38 : location_info := LocationInfo file_0 62 6 62 15.
-  Definition loc_39 : location_info := LocationInfo file_0 62 7 62 10.
-  Definition loc_40 : location_info := LocationInfo file_0 62 18 62 27.
-  Definition loc_41 : location_info := LocationInfo file_0 62 18 62 27.
-  Definition loc_42 : location_info := LocationInfo file_0 62 19 62 22.
-  Definition loc_43 : location_info := LocationInfo file_0 61 2 61 11.
-  Definition loc_44 : location_info := LocationInfo file_0 61 3 61 6.
-  Definition loc_45 : location_info := LocationInfo file_0 61 2 61 29.
-  Definition loc_46 : location_info := LocationInfo file_0 61 2 61 11.
-  Definition loc_47 : location_info := LocationInfo file_0 61 2 61 11.
-  Definition loc_48 : location_info := LocationInfo file_0 61 3 61 6.
-  Definition loc_49 : location_info := LocationInfo file_0 61 15 61 29.
-  Definition loc_50 : location_info := LocationInfo file_0 61 15 61 23.
-  Definition loc_51 : location_info := LocationInfo file_0 61 15 61 23.
-  Definition loc_52 : location_info := LocationInfo file_0 61 27 61 29.
-  Definition loc_53 : location_info := LocationInfo file_0 59 4 59 26.
-  Definition loc_54 : location_info := LocationInfo file_0 59 11 59 25.
-  Definition loc_56 : location_info := LocationInfo file_0 58 6 58 15.
-  Definition loc_58 : location_info := LocationInfo file_0 58 7 58 15.
-  Definition loc_59 : location_info := LocationInfo file_0 58 7 58 15.
-  Definition loc_60 : location_info := LocationInfo file_0 55 18 55 27.
-  Definition loc_61 : location_info := LocationInfo file_0 55 18 55 27.
-  Definition loc_62 : location_info := LocationInfo file_0 55 19 55 22.
-  Definition loc_67 : location_info := LocationInfo file_0 83 2 83 35.
-  Definition loc_68 : location_info := LocationInfo file_0 83 9 83 34.
-  Definition loc_69 : location_info := LocationInfo file_0 83 9 83 31.
-  Definition loc_70 : location_info := LocationInfo file_0 83 9 83 31.
-  Definition loc_71 : location_info := LocationInfo file_0 83 32 83 33.
-  Definition loc_74 : location_info := LocationInfo file_0 93 2 93 20.
-  Definition loc_75 : location_info := LocationInfo file_0 94 2 94 52.
-  Definition loc_76 : location_info := LocationInfo file_0 95 2 95 31.
-  Definition loc_77 : location_info := LocationInfo file_0 95 2 95 11.
-  Definition loc_78 : location_info := LocationInfo file_0 95 3 95 6.
-  Definition loc_79 : location_info := LocationInfo file_0 95 14 95 30.
-  Definition loc_80 : location_info := LocationInfo file_0 95 26 95 30.
-  Definition loc_81 : location_info := LocationInfo file_0 95 26 95 30.
-  Definition loc_82 : location_info := LocationInfo file_0 94 2 94 11.
-  Definition loc_83 : location_info := LocationInfo file_0 94 3 94 6.
-  Definition loc_84 : location_info := LocationInfo file_0 94 14 94 51.
-  Definition loc_85 : location_info := LocationInfo file_0 94 26 94 51.
-  Definition loc_86 : location_info := LocationInfo file_0 94 27 94 43.
-  Definition loc_87 : location_info := LocationInfo file_0 94 39 94 43.
-  Definition loc_88 : location_info := LocationInfo file_0 94 39 94 43.
-  Definition loc_89 : location_info := LocationInfo file_0 94 46 94 50.
-  Definition loc_90 : location_info := LocationInfo file_0 94 46 94 50.
-  Definition loc_91 : location_info := LocationInfo file_0 93 2 93 12.
-  Definition loc_92 : location_info := LocationInfo file_0 93 3 93 6.
-  Definition loc_93 : location_info := LocationInfo file_0 93 15 93 19.
-  Definition loc_94 : location_info := LocationInfo file_0 93 15 93 19.
+  Definition loc_2 : location_info := LocationInfo file_0 41 2 41 52.
+  Definition loc_3 : location_info := LocationInfo file_0 41 9 41 51.
+  Definition loc_4 : location_info := LocationInfo file_0 41 9 41 45.
+  Definition loc_5 : location_info := LocationInfo file_0 41 10 41 19.
+  Definition loc_6 : location_info := LocationInfo file_0 41 10 41 19.
+  Definition loc_7 : location_info := LocationInfo file_0 41 11 41 14.
+  Definition loc_8 : location_info := LocationInfo file_0 41 22 41 44.
+  Definition loc_9 : location_info := LocationInfo file_0 41 34 41 44.
+  Definition loc_10 : location_info := LocationInfo file_0 41 34 41 44.
+  Definition loc_11 : location_info := LocationInfo file_0 41 35 41 38.
+  Definition loc_12 : location_info := LocationInfo file_0 41 49 41 51.
+  Definition loc_15 : location_info := LocationInfo file_0 57 2 57 31.
+  Definition loc_16 : location_info := LocationInfo file_0 60 2 61 26.
+  Definition loc_17 : location_info := LocationInfo file_0 63 2 63 30.
+  Definition loc_18 : location_info := LocationInfo file_0 64 2 67 3.
+  Definition loc_19 : location_info := LocationInfo file_0 75 2 75 67.
+  Definition loc_20 : location_info := LocationInfo file_0 75 9 75 66.
+  Definition loc_21 : location_info := LocationInfo file_0 75 35 75 47.
+  Definition loc_22 : location_info := LocationInfo file_0 75 35 75 47.
+  Definition loc_23 : location_info := LocationInfo file_0 75 37 75 40.
+  Definition loc_24 : location_info := LocationInfo file_0 75 51 75 65.
+  Definition loc_25 : location_info := LocationInfo file_0 75 61 75 64.
+  Definition loc_26 : location_info := LocationInfo file_0 75 61 75 64.
+  Definition loc_27 : location_info := LocationInfo file_0 64 29 67 3.
+  Definition loc_28 : location_info := LocationInfo file_0 65 4 65 20.
+  Definition loc_29 : location_info := LocationInfo file_0 66 4 66 26.
+  Definition loc_30 : location_info := LocationInfo file_0 66 11 66 25.
+  Definition loc_31 : location_info := LocationInfo file_0 65 4 65 13.
+  Definition loc_32 : location_info := LocationInfo file_0 65 5 65 8.
+  Definition loc_33 : location_info := LocationInfo file_0 65 16 65 19.
+  Definition loc_34 : location_info := LocationInfo file_0 65 16 65 19.
+  Definition loc_36 : location_info := LocationInfo file_0 64 6 64 27.
+  Definition loc_37 : location_info := LocationInfo file_0 64 6 64 15.
+  Definition loc_38 : location_info := LocationInfo file_0 64 6 64 15.
+  Definition loc_39 : location_info := LocationInfo file_0 64 7 64 10.
+  Definition loc_40 : location_info := LocationInfo file_0 64 18 64 27.
+  Definition loc_41 : location_info := LocationInfo file_0 64 18 64 27.
+  Definition loc_42 : location_info := LocationInfo file_0 64 19 64 22.
+  Definition loc_43 : location_info := LocationInfo file_0 63 2 63 11.
+  Definition loc_44 : location_info := LocationInfo file_0 63 3 63 6.
+  Definition loc_45 : location_info := LocationInfo file_0 63 2 63 29.
+  Definition loc_46 : location_info := LocationInfo file_0 63 2 63 11.
+  Definition loc_47 : location_info := LocationInfo file_0 63 2 63 11.
+  Definition loc_48 : location_info := LocationInfo file_0 63 3 63 6.
+  Definition loc_49 : location_info := LocationInfo file_0 63 15 63 29.
+  Definition loc_50 : location_info := LocationInfo file_0 63 15 63 23.
+  Definition loc_51 : location_info := LocationInfo file_0 63 15 63 23.
+  Definition loc_52 : location_info := LocationInfo file_0 63 27 63 29.
+  Definition loc_53 : location_info := LocationInfo file_0 61 4 61 26.
+  Definition loc_54 : location_info := LocationInfo file_0 61 11 61 25.
+  Definition loc_56 : location_info := LocationInfo file_0 60 6 60 15.
+  Definition loc_58 : location_info := LocationInfo file_0 60 7 60 15.
+  Definition loc_59 : location_info := LocationInfo file_0 60 7 60 15.
+  Definition loc_60 : location_info := LocationInfo file_0 57 18 57 27.
+  Definition loc_61 : location_info := LocationInfo file_0 57 18 57 27.
+  Definition loc_62 : location_info := LocationInfo file_0 57 19 57 22.
+  Definition loc_67 : location_info := LocationInfo file_0 85 2 85 16.
+  Definition loc_68 : location_info := LocationInfo file_0 85 16 85 3.
+  Definition loc_69 : location_info := LocationInfo file_0 86 2 86 35.
+  Definition loc_70 : location_info := LocationInfo file_0 86 9 86 34.
+  Definition loc_71 : location_info := LocationInfo file_0 86 9 86 31.
+  Definition loc_72 : location_info := LocationInfo file_0 86 9 86 31.
+  Definition loc_73 : location_info := LocationInfo file_0 86 32 86 33.
+  Definition loc_74 : location_info := LocationInfo file_0 85 2 85 15.
+  Definition loc_75 : location_info := LocationInfo file_0 85 3 85 15.
+  Definition loc_76 : location_info := LocationInfo file_0 85 5 85 8.
+  Definition loc_79 : location_info := LocationInfo file_0 96 2 96 20.
+  Definition loc_80 : location_info := LocationInfo file_0 97 2 97 52.
+  Definition loc_81 : location_info := LocationInfo file_0 98 2 98 31.
+  Definition loc_82 : location_info := LocationInfo file_0 98 2 98 11.
+  Definition loc_83 : location_info := LocationInfo file_0 98 3 98 6.
+  Definition loc_84 : location_info := LocationInfo file_0 98 14 98 30.
+  Definition loc_85 : location_info := LocationInfo file_0 98 26 98 30.
+  Definition loc_86 : location_info := LocationInfo file_0 98 26 98 30.
+  Definition loc_87 : location_info := LocationInfo file_0 97 2 97 11.
+  Definition loc_88 : location_info := LocationInfo file_0 97 3 97 6.
+  Definition loc_89 : location_info := LocationInfo file_0 97 14 97 51.
+  Definition loc_90 : location_info := LocationInfo file_0 97 26 97 51.
+  Definition loc_91 : location_info := LocationInfo file_0 97 27 97 43.
+  Definition loc_92 : location_info := LocationInfo file_0 97 39 97 43.
+  Definition loc_93 : location_info := LocationInfo file_0 97 39 97 43.
+  Definition loc_94 : location_info := LocationInfo file_0 97 46 97 50.
+  Definition loc_95 : location_info := LocationInfo file_0 97 46 97 50.
+  Definition loc_96 : location_info := LocationInfo file_0 96 2 96 12.
+  Definition loc_97 : location_info := LocationInfo file_0 96 3 96 6.
+  Definition loc_98 : location_info := LocationInfo file_0 96 15 96 19.
+  Definition loc_99 : location_info := LocationInfo file_0 96 15 96 19.
 
   (* Definition of struct [region]. *)
   Program Definition struct_region := {|
     sl_members := [
-      (Some "base", void*);
       (Some "end", it_layout size_t);
-      (Some "cur", it_layout size_t)
+      (Some "cur", it_layout size_t);
+      (Some "base", void*)
     ];
   |}.
   Solve Obligations with solve_struct_obligations.
@@ -178,7 +183,7 @@ Section code.
   |}.
 
   (* Definition of function [hyp_early_alloc_page]. *)
-  Definition impl_hyp_early_alloc_page (global_hyp_early_alloc_contig : loc): function := {|
+  Definition impl_hyp_early_alloc_page (global_mem global_hyp_early_alloc_contig : loc): function := {|
     f_args := [
       ("arg", void*)
     ];
@@ -188,7 +193,9 @@ Section code.
     f_code := (
       <[ "#0" :=
         locinfo: loc_67 ;
-        Return (LocInfoE loc_68 (Call (LocInfoE loc_70 (global_hyp_early_alloc_contig)) [@{expr} LocInfoE loc_71 (UnOp (CastOp $ IntOp u32) (IntOp i32) (LocInfoE loc_71 (i2v 1 i32))) ]))
+        expr: (LocInfoE loc_74 (&(LocInfoE loc_75 ((LocInfoE loc_76 (global_mem)) at{struct_region} "base")))) ;
+        locinfo: loc_69 ;
+        Return (LocInfoE loc_70 (Call (LocInfoE loc_72 (global_hyp_early_alloc_contig)) [@{expr} LocInfoE loc_73 (UnOp (CastOp $ IntOp u32) (IntOp i32) (LocInfoE loc_73 (i2v 1 i32))) ]))
       ]> $∅
     )%E
   |}.
@@ -204,15 +211,15 @@ Section code.
     f_init := "#0";
     f_code := (
       <[ "#0" :=
-        locinfo: loc_74 ;
-        LocInfoE loc_91 ((LocInfoE loc_92 (global_mem)) at{struct_region} "base") <-{ void* }
-          LocInfoE loc_93 (use{void*} (LocInfoE loc_94 ("virt"))) ;
-        locinfo: loc_75 ;
-        LocInfoE loc_82 ((LocInfoE loc_83 (global_mem)) at{struct_region} "end") <-{ it_layout size_t }
-          LocInfoE loc_84 (UnOp (CastOp $ IntOp size_t) (IntOp size_t) (LocInfoE loc_85 ((LocInfoE loc_86 (UnOp (CastOp $ IntOp size_t) (PtrOp) (LocInfoE loc_87 (use{void*} (LocInfoE loc_88 ("virt")))))) +{IntOp size_t, IntOp size_t} (LocInfoE loc_89 (UnOp (CastOp $ IntOp size_t) (IntOp u32) (LocInfoE loc_89 (use{it_layout u32} (LocInfoE loc_90 ("size"))))))))) ;
-        locinfo: loc_76 ;
-        LocInfoE loc_77 ((LocInfoE loc_78 (global_mem)) at{struct_region} "cur") <-{ it_layout size_t }
-          LocInfoE loc_79 (UnOp (CastOp $ IntOp size_t) (PtrOp) (LocInfoE loc_80 (use{void*} (LocInfoE loc_81 ("virt"))))) ;
+        locinfo: loc_79 ;
+        LocInfoE loc_96 ((LocInfoE loc_97 (global_mem)) at{struct_region} "base") <-{ void* }
+          LocInfoE loc_98 (use{void*} (LocInfoE loc_99 ("virt"))) ;
+        locinfo: loc_80 ;
+        LocInfoE loc_87 ((LocInfoE loc_88 (global_mem)) at{struct_region} "end") <-{ it_layout size_t }
+          LocInfoE loc_89 (UnOp (CastOp $ IntOp size_t) (IntOp size_t) (LocInfoE loc_90 ((LocInfoE loc_91 (UnOp (CastOp $ IntOp size_t) (PtrOp) (LocInfoE loc_92 (use{void*} (LocInfoE loc_93 ("virt")))))) +{IntOp size_t, IntOp size_t} (LocInfoE loc_94 (UnOp (CastOp $ IntOp size_t) (IntOp u32) (LocInfoE loc_94 (use{it_layout u32} (LocInfoE loc_95 ("size"))))))))) ;
+        locinfo: loc_81 ;
+        LocInfoE loc_82 ((LocInfoE loc_83 (global_mem)) at{struct_region} "cur") <-{ it_layout size_t }
+          LocInfoE loc_84 (UnOp (CastOp $ IntOp size_t) (PtrOp) (LocInfoE loc_85 (use{void*} (LocInfoE loc_86 ("virt"))))) ;
         Return (VOID)
       ]> $∅
     )%E
