linux/pkvm/proofs/early_alloc/generated_proof_hyp_early_alloc_nr_pages.v
@@ -1,1 +1,30 @@
-(* Let's skip that, you seem to have some faith. *)
+From refinedc.typing Require Import typing.
+From refinedc.linux.pkvm.early_alloc Require Import generated_code.
+From refinedc.linux.pkvm.early_alloc Require Import generated_spec.
+From refinedc.linux.pkvm.early_alloc Require Import instances.
+Set Default Proof Using "Type".
+
+(* Generated from [linux/pkvm/early_alloc.c]. *)
+Section proof_hyp_early_alloc_nr_pages.
+  Context `{!typeG Σ} `{!globalG Σ}.
+
+  (* Typing proof for [hyp_early_alloc_nr_pages]. *)
+  Lemma type_hyp_early_alloc_nr_pages (global_mem : loc) :
+    global_locs !! "mem" = Some global_mem →
+    ⊢ typed_function (impl_hyp_early_alloc_nr_pages global_mem) type_of_hyp_early_alloc_nr_pages.
+  Proof.
+    Open Scope printing_sugar.
+    start_function "hyp_early_alloc_nr_pages" ([[base given] remaining]).
+    split_blocks ((
+      ∅
+    )%I : gmap label (iProp Σ)) ((
+      ∅
+    )%I : gmap label (iProp Σ)).
+    - repeat liRStep; liShow.
+      all: print_typesystem_goal "hyp_early_alloc_nr_pages" "#0".
+    Unshelve. all: sidecond_hook; prepare_sideconditions; normalize_and_simpl_goal; try solve_goal; unsolved_sidecond_hook.
+    + rewrite Z.add_simpl_l /PAGE_SIZE. solve_goal.
+    + rewrite /PAGE_SIZE Z.add_simpl_l Z.shiftr_div_pow2 //= Z.div_mul //=.
+    all: print_sidecondition_goal "hyp_early_alloc_nr_pages".
+  Qed.
+End proof_hyp_early_alloc_nr_pages.
