linux/pkvm/proofs/early_alloc/instances.v
@@ -1,6 +1,8 @@
 From refinedc.typing Require Import typing.
 Set Default Proof Using "Type".
 
+Remove Hints find_in_context_type_val_P_own_singleton_inst : typeclass_instances.
+
 Section instances.
   Context  `{!typeG Σ}.
 
@@ -34,4 +36,41 @@ Section instances.
   Global Instance simplify_goal_place_combine_offset_inst l β n ty:
     SimplifyGoalPlace (l.1, l.2 + n) β ty (Some 0%N) :=
     λ T, i2p (simplify_goal_place_combine_offset l β n ty T).
+
+  Lemma type_cast_ptr_int_val (v : val) (p : loc) (n : nat) T:
+    (⌜min_alloc_start ≤ p.2 ∧ p.2 + n ≤ max_alloc_end⌝ -∗
+      v ◁ᵥ p @ ptr n -∗ T (i2v p.2 size_t) (t2mt (p.2 @ int uintptr_t))) -∗
+    typed_un_op v (v ◁ᵥ p @ ptr n) (CastOp (IntOp uintptr_t)) PtrOp T.
+  Proof.
+    iIntros "HT Hp" (Φ) "HΦ".
+    iDestruct "Hp" as "[-> #Hlib]".
+    iDestruct (loc_in_bounds_in_range_uintptr_t with "Hlib") as %[? H]%val_of_int_is_some.
+    iDestruct (loc_in_bounds_ptr_in_range with "Hlib") as %?.
+    iDestruct ("HT" with "[] []") as "HT"; first done. { by iFrame "Hlib". }
+    iApply wp_cast_ptr_int => //=; first by rewrite val_to_of_loc.
+    rewrite /i2v H /=. iApply ("HΦ" with "[] [HT]"); last done. done.
+  Qed.
+  Global Instance type_cast_ptr_int_val_inst (v : val) (p : loc) n:
+    TypedUnOp v (v ◁ᵥ p @ ptr n)%I (CastOp (IntOp uintptr_t)) PtrOp :=
+    λ T, i2p (type_cast_ptr_int_val v p n T).
+
+  Lemma subsume_own_ptr p l1 l2 ty n T:
+    ⌜l1 = l2⌝ ∗ (l1 ◁ₗ ty -∗ loc_in_bounds l1 n ∗ T) -∗
+    subsume (p ◁ₗ l1 @ &own ty)%I (p ◁ₗ l2 @ ptr n)%I T.
+  Proof.
+    iIntros "[-> HT] Hp".
+    iDestruct (ty_aligned with "Hp") as %?.
+    iDestruct (ty_deref with "Hp") as (v) "[Hp [-> Hl]]".
+    iDestruct ("HT" with "Hl") as "[#Hlib $]".
+    iFrame "Hp Hlib". done.
+  Qed.
+  Global Instance subsume_own_ptr_inst p l1 l2 ty n:
+    Subsume (p ◁ₗ l1 @ &own ty)%I (p ◁ₗ l2 @ ptr n)%I :=
+    λ T, i2p (subsume_own_ptr p l1 l2 ty n T).
+
+  Global Instance intro_persistent_loc_in_bounds l n:
+    IntroPersistent (loc_in_bounds l n) (loc_in_bounds l n).
+  Proof. constructor. by iIntros "#H !>". Qed.
 End instances.
+
+Typeclasses Opaque FindLocInBounds.
